theories/mlanguage/adequacy.v
@@ -1,0 +1,116 @@
+From iris.proofmode Require Import base proofmode classes.
+From transfinite.base_logic.lib Require Export fancy_updates.
+From melocoton.mlanguage Require Export mlanguage progenv weakestpre.
+From melocoton Require Import multirelations named_props.
+From iris.bi Require Export weakestpre.
+From iris.prelude Require Import options.
+From transfinite.base_logic.lib Require Import satisfiable.
+From transfinite.stepindex Require Import ordinals.
+Import uPred.
+Import umrel.
+
+Section Adequacy.
+  Existing Instance ordI.
+  Context {val : Type}.
+  Context {Λ : mlanguage val}.
+  Context {Σ : gFunctors}.
+
+  Context {Φpure : val → state Λ → Prop}.
+  Context {pe : prog_environ Λ Σ}.
+  Context {Φbi : val → iProp Σ}.
+
+  Notation step := (prim_step (penv_prog pe)).
+  Notation cfg := (prod (expr Λ) (state Λ)).
+
+  Implicit Types σ : state Λ.
+  Implicit Types v : val.
+  Implicit Types e : expr Λ.
+  Implicit Types X : cfg → Prop.
+
+
+
+  Section GenAdequacy.
+    Context {sat_at : coPset → iProp Σ → Prop}.
+    Context `{!invG Σ, !mlangG val Λ Σ}.
+    Context `{!SatisfiableAt sat_at}.
+    Context `{SatisfiableAtExists (cfg→Prop) sat_at}.
+
+    (* XXX this can be strengthened to allow opening invariants (without needing to close them again annoyingly) *)
+    Hypothesis HΦ : (⊢ ∀ σ v, state_interp σ ∗ Φbi v ==∗ ⌜Φpure v σ⌝).
+    Hypothesis Hpeclosed : (⊢ ∀ f s vv, penv_proto pe f s vv -∗ False).
+
+    Lemma value_from_wp σ v E :
+      sat_at E (state_interp σ ∗ WP (of_val Λ v) @ pe; E {{Φbi}})%I
+    → Φpure v σ.
+    Proof using All.
+      intros Hsat. eapply sat_mono in Hsat.
+      2: {
+        iIntros "(Hσ&HWP)".
+        rewrite wp_unfold /wp_pre.
+        iPoseProof ("HWP" $! σ with "Hσ") as "HWP". iAccu. }
+      eapply sat_fupd, sat_mono in Hsat.
+      2: { iIntros "[(%z & %HH & H)|[(%s & %vv & %K & %is_call & H2 & Hb & Hσ & (%Ξ & Hprot & _))|(%Hnv&_)]]".
+        - apply of_val_inj in HH. subst z.
+          iPoseProof (HΦ $! σ v with "H") as "H". iAccu.
+        - iExFalso. iApply Hpeclosed. iApply "Hprot".
+        - by rewrite to_of_val in Hnv. }
+      by eapply sat_bupd, sat_elim in Hsat.
+    Qed.
+
+    Lemma one_step_from_wp σ e E:
+      (to_val e = None) →
+      sat_at E (state_interp σ ∗ WP e @ pe; E {{Φbi}})%I →
+      ∃ X, step (e,σ) X ∧ ∀ e' σ', X (e', σ') → sat_at E (state_interp σ' ∗ WP e' @ pe; E {{Φbi}}).
+    Proof using All.
+      intros Hnv Hsat.
+      eapply sat_mono in Hsat.
+      2: {
+        iIntros "(Hσ&HWP)".
+        rewrite wp_unfold /wp_pre.
+        iPoseProof ("HWP" $! σ with "Hσ") as "HWP". iAccu. }
+      eapply sat_fupd, sat_mono in Hsat.
+      2: { iIntros "[(%z & %HH & H)|[(%s & %vv & %K & %is_call & H2 & Hb & Hσ & (%Ξ & Hprot & _))|(_&H3)]]".
+        - subst e. by rewrite to_of_val in Hnv.
+        - iExFalso. iApply Hpeclosed. iApply "Hprot".
+        - iAccu. }
+      eapply sat_exists in Hsat. destruct Hsat as (X&(Hstep%sat_elim&Hsat)%sat_sep).
+      exists X; split; first done.
+      intros e' σ' Hcfg'.
+      eapply (sat_forall e'), (sat_forall σ'), sat_wand in Hsat.
+      2: iIntros "_"; by iPureIntro.
+      eapply sat_fupd, sat_later, sat_fupd in Hsat. done.
+    Qed.
+
+    Lemma star_step_from_wp σ e E X:
+      sat_at E (state_interp σ ∗ WP e @ pe; E {{Φbi}})%I →
+      (star_AD step (e, σ) X) →
+      (∃ e σ, X (e, σ) ∧ (∀ v, to_val e = Some v → Φpure v σ)).
+    Proof using All.
+      assert (∃ x, fst x = e ∧ snd x = σ ∧ (e,σ)=x) as (x&<-&<-&->).
+      1: by exists (e,σ).
+      intros Hsat. unfold mrel; cbn in *.
+      induction 1 as [[e σ] X H|[e σ] X IH] in Hsat|-*; cbn in *.
+      - exists e, σ. split; first done.
+        intros v <-%of_to_val. by eapply value_from_wp.
+      - destruct (to_val e) as [v|] eqn:Heq.
+        1: eapply of_to_val in Heq; subst e;
+          destruct (IH _ (val_prim_step _ _ _)) as (?&[]&_).
+        eapply one_step_from_wp in Hsat; last done.
+        destruct Hsat as (Y&HstepY&Hcont).
+        destruct (IH Y HstepY) as ([e' σ']&Hy&Hmrel&Hsat).
+        eapply Hsat, Hcont, Hy.
+    Qed.
+
+  End GenAdequacy.
+
+  Section ConreteAdequacy.
+    Context `{!invGpreS Σ}.
+  
+
+  End ConreteAdequacy.
+End Adequacy.
+
+
+
+
+
